reorg
- clean up the ExprUVar and ExprVar interfaces

theories/VariablesI.v
@@ -1,9 +1,13 @@
+Require Import Coq.Bool.Bool.
 Require Import Coq.Lists.List.
+Require Import Coq.Classes.Morphisms.
+Require Import ExtLib.Core.RelDec.
 Require Import ExtLib.Data.HList.
 Require Import ExtLib.Tactics.
 Require Import MirrorCore.TypesI.
 Require Import MirrorCore.ExprI.
 Require Import MirrorCore.EnvI.
+Require Import MirrorCore.CtxLogic.
 
 Set Implicit Arguments.
 Set Strict Implicit.
@@ -16,8 +20,8 @@ Section with_Expr.
   Context {Expr_expr : @Expr typ _ expr}.
 
   Class ExprVar : Type :=
-  { Var : nat -> expr
-  ; mentionsV : nat -> expr -> bool
+  { Var : var -> expr
+  ; mentionsV : var -> expr -> bool
   }.
 
   Class ExprVarOk (EV : ExprVar) : Prop :=
@@ -69,9 +73,61 @@ Section with_Expr.
   Qed.
 
   Class ExprUVar : Type :=
-  { UVar : nat -> expr
-  ; mentionsU : nat -> expr -> bool
+  { UVar : uvar -> expr
+  ; mentionsU : uvar -> expr -> bool
+  ; instantiate : (uvar -> option expr) -> nat -> expr -> expr
   }.
+
+
+  Definition sem_preserves_if_ho tus tvs
+             (P : exprT tus tvs Prop -> Prop)
+             (f : uvar -> option expr) : Prop :=
+    forall u e t get,
+      f u = Some e ->
+      nth_error_get_hlist_nth _ tus u = Some (@existT _ _ t get) ->
+      exists eD,
+        exprD' tus tvs e t = Some eD /\
+        P (fun us vs => get us = eD us vs).
+
+  Definition sem_preserves_if tus tvs
+             (P : exprT tus tvs Prop)
+             (f : uvar -> option expr) : Prop :=
+    @sem_preserves_if_ho tus tvs
+                         (fun P' => forall us vs, P us vs -> P' us vs) f.
+
+  Definition instantiate_spec_ho
+             (instantiate : (uvar -> option expr) -> nat -> expr -> expr)
+  : Prop :=
+    forall tus tvs f e tvs' t eD P (EApp : CtxLogic.ExprTApplicative P),
+      sem_preserves_if_ho P f ->
+      exprD' tus (tvs' ++ tvs) e t = Some eD ->
+      exists eD',
+        exprD' tus (tvs' ++ tvs) (instantiate f (length tvs') e) t = Some eD' /\
+        P (fun us vs => forall vs',
+                          eD us (hlist_app vs' vs) = eD' us (hlist_app vs' vs)).
+
+  Definition instantiate_spec
+             (instantiate : (uvar -> option expr) -> nat -> expr -> expr)
+  : Prop :=
+    forall tus tvs f e tvs' t eD P,
+      @sem_preserves_if tus tvs P f ->
+      exprD' tus (tvs' ++ tvs) e t = Some eD ->
+      exists eD',
+        exprD' tus (tvs' ++ tvs) (instantiate f (length tvs') e) t = Some eD' /\
+        forall us vs vs', P us vs ->
+          eD us (hlist_app vs' vs) = eD' us (hlist_app vs' vs).
+
+  Definition instantiate_mentionsU_spec
+             (instantiate : (uvar -> option expr) -> nat -> expr -> expr)
+             (mentionsU : uvar -> expr -> bool)
+  : Prop :=
+    forall f n e u,
+      mentionsU u (instantiate f n e) = true <-> (** do i need iff? **)
+      (   (f u = None /\ mentionsU u e = true)
+       \/ exists u' e',
+            f u' = Some e' /\
+            mentionsU u' e = true /\
+            mentionsU u e' = true).
 
   Class ExprUVarOk (EU : ExprUVar) : Prop :=
   { UVar_exprD'
@@ -95,7 +151,18 @@ Section with_Expr.
         forall us vs u,
           val (hlist_app us (Hcons u Hnil)) vs = val' us vs
   ; mentionsU_UVar : forall v v', mentionsU v (UVar v') = true <-> v = v'
+  ; instantiate_mentionsU : instantiate_mentionsU_spec instantiate mentionsU
+  ; instantiate_sound_ho : instantiate_spec_ho instantiate
   }.
+
+  Theorem instantiate_sound (EU : ExprUVar) (EUO : ExprUVarOk EU)
+  : instantiate_spec instantiate.
+  Proof.
+    red; intros.
+    eapply (@instantiate_sound_ho _ EUO) in H0; try eassumption.
+    - forward_reason; eauto.
+    - eapply (ExprTApplicative_foralls_impl).
+  Qed.
 
   Lemma exprD'_exact_uvar {EU} {EUO : ExprUVarOk EU} tus tus' tvs t
   : exists eD' : exprT (tus ++ t :: tus') tvs (typD t),
@@ -121,9 +188,30 @@ Section with_Expr.
       inversion H. apply H0. assumption. }
   Qed.
 
+  Class MentionsAny : Type :=
+  { mentionsAny : (uvar -> bool) -> (var -> bool) -> expr -> bool }.
+
+  Class MentionsAnyOk (MA : MentionsAny) (MV : ExprVar) (MU : ExprUVar) : Type :=
+  { Proper_mentionsAny
+    : Proper ((eq ==> eq) ==> (eq ==> eq) ==> eq ==> eq) mentionsAny
+  ; mentionsAny_factor
+    : forall fu fu' fv fv' e,
+          mentionsAny (fun u => fu u || fu' u) (fun v => fv v || fv' v) e
+        = mentionsAny fu fv e || mentionsAny fu' fv' e
+  ; mentionsAny_mentionsU
+    : forall u e, mentionsU u e = mentionsAny (fun u' => u ?[ eq ] u') (fun _ => false) e
+  }.
+
 End with_Expr.
 
 Arguments ExprVar expr : rename.
 Arguments ExprUVar expr : rename.
 Arguments ExprVarOk {typ _ expr _} _ : rename.
 Arguments ExprUVarOk {typ _ expr _} _ : rename.
+Arguments instantiate {expr ExprUVar} _ _ _ : rename.
+Arguments mentionsU {expr ExprUVar} _ _ : rename.
+Arguments mentionsV {expr ExprVar} _ _ : rename.
+Arguments mentionsAny {expr MentionsAny} _ _ _ : rename.
+Arguments instantiate_sound {typ expr RType Expr EU EUO} _ _ _ _ tvs' _ _ P _ _ : rename.
+Arguments instantiate_sound_ho {typ expr RType Expr EU EUO} _ _ _ _ tvs' _ _ P _ _ _ : rename.
+Arguments instantiate_mentionsU {typ expr RType Expr EU EUO} _ _ _ _ : rename.
