theories/RTac/Apply.v
@@ -20,15 +20,19 @@ Section parameterized.
 
   Context {RType_typ : RType typ}.
   Context {RTypeOk_typ : RTypeOk}.
+  Context {Typ0_Prop : Typ0 _ Prop}.
   Context {Expr_expr : Expr RType_typ expr}.
   Context {ExprOk_expr : ExprOk Expr_expr}.
-  Context {Typ0_Prop : Typ0 _ Prop}.
+  Context {ExprVar_expr : ExprVar expr}.
+  Context {ExprVarOk_expr : ExprVarOk _}.
   Context {ExprUVar_expr : ExprUVar expr}.
+  Context {ExprUVarOk_expr : ExprUVarOk _}.
+  Context {MentionsAny_expr : MentionsAny expr}.
+  Context {MentionsAnyOk_expr : MentionsAnyOk _ _ _}.
 
   Variable vars_to_uvars : nat -> nat -> expr -> expr.
   Variable exprUnify : forall subst, Subst subst expr -> SubstUpdate subst expr ->
     tenv typ -> tenv typ -> nat -> expr -> expr -> typ -> subst -> option subst.
-  Variable instantiate : (nat -> option expr) -> nat -> expr -> expr.
 
   Variable vars_to_uvars_sound : vars_to_uvars_spec vars_to_uvars.
   Variable exprUnify_sound
@@ -39,7 +43,7 @@ Section parameterized.
   Variable lem : Lemma.lemma typ expr expr.
 
   Definition APPLY : rtac typ expr :=
-    @EAPPLY typ expr _ _ _ vars_to_uvars exprUnify instantiate lem.
+    @EAPPLY typ expr _ _ _ _ vars_to_uvars exprUnify lem.
 
   Hypothesis lemD :
     @Lemma.lemmaD typ expr _ _ expr (@exprD'_typ0 _ _ _ _ Prop _)
